Finish recovery adequacy for new crash wp.

src/program_logic/recovery_adequacy.v
@@ -7,56 +7,66 @@ Import uPred.
 
 Section crash_adequacy.
 Context `{!irisG Λ Σ}.
+Implicit Types s : stuckness.
+Implicit Types k : nat.
 Implicit Types e : expr Λ.
 Implicit Types P Q : iProp Σ.
 Implicit Types Φ : val Λ → iProp Σ.
 Implicit Types Φs : list (val Λ → iProp Σ).
 
-Notation wptp s t := ([∗ list] ef ∈ t, WPC ef @ s; ⊤; ∅ {{ fork_post }} {{ True }})%I.
+Notation wptp s k t := ([∗ list] ef ∈ t, WPC ef @ s; k; ⊤; ∅ {{ fork_post }} {{ True }})%I.
 
-Lemma wpc_step s e1 σ1 κ κs e2 σ2 efs m Φ Φc :
+Lemma wpc_step s k e1 σ1 κ κs e2 σ2 efs m Φ Φc :
   prim_step e1 σ1 κ e2 σ2 efs →
-  state_interp σ1 (κ ++ κs) m -∗ WPC e1 @ s; ⊤; ∅ {{ Φ }} {{ Φc }} ={⊤,∅}▷=∗
+  state_interp σ1 (κ ++ κs) m -∗ WPC e1 @ s; k; ⊤; ∅ {{ Φ }} {{ Φc }} -∗
+  |={⊤,⊤}_(2 * (S (S k)))=>
   state_interp σ2 κs (length efs + m) ∗
-  WPC e2 @ s; ⊤; ∅ {{ Φ }} {{ Φc }} ∗
-  wptp s efs.
+  WPC e2 @ s; k; ⊤; ∅ {{ Φ }} {{ Φc }} ∗
+  wptp s k efs.
 Proof.
   rewrite {1}wpc_unfold /wpc_pre. iIntros (?) "Hσ H".
   rewrite (val_stuck e1 σ1 κ e2 σ2 efs) //.
   iDestruct "H" as "(H&_)".
-  iMod ("H" $! σ1 with "Hσ") as "(_ & H)".
+  replace (2 * S (S k)) with (S (S k) + S (S k)) by lia.
+  rewrite Nat_iter_add Nat_iter_S.
+  iMod ("H" $! σ1 with "Hσ") as "H".
+  do 4 iModIntro. iApply (step_fupdN_wand with "H").
+  iIntros "(H&_)". rewrite Nat_iter_S.
+  iMod "H" as "(_ & H)".
   iMod ("H" $! e2 σ2 efs with "[//]") as "H".
-  by iIntros "!> !>".
+  iIntros "!> !>". by iMod "H".
 Qed.
 
-Lemma wptp_step s e1 t1 t2 κ κs σ1 σ2 Φ Φc :
+Lemma wptp_step s k e1 t1 t2 κ κs σ1 σ2 Φ Φc :
   step (e1 :: t1,σ1) κ (t2, σ2) →
-  state_interp σ1 (κ ++ κs) (length t1) -∗ WPC e1 @ s; ⊤; ∅ {{ Φ }} {{ Φc }}-∗ wptp s t1 ==∗
+  state_interp σ1 (κ ++ κs) (length t1) -∗ WPC e1 @ s; k; ⊤; ∅ {{ Φ }} {{ Φc }}-∗ wptp s k t1 ==∗
   ∃ e2 t2', ⌜t2 = e2 :: t2'⌝ ∗
-  |={⊤,∅}▷=> state_interp σ2 κs (pred (length t2)) ∗ WPC e2 @ s; ⊤; ∅ {{ Φ }} {{ Φc}}  ∗ wptp s t2'.
+  |={⊤,⊤}_(2 * (S (S k)))=> state_interp σ2 κs (pred (length t2)) ∗ WPC e2 @ s; k; ⊤; ∅ {{ Φ }} {{ Φc}} ∗ wptp s k t2'.
 Proof.
   iIntros (Hstep) "Hσ He Ht".
   destruct Hstep as [e1' σ1' e2' σ2' efs [|? t1'] t2' ?? Hstep]; simplify_eq/=.
   - iExists e2', (t2' ++ efs). iModIntro. iSplitR; first by eauto.
     iMod (wpc_step with "Hσ He") as "H"; first done.
-    iIntros "!> !>". iMod "H" as "(Hσ & He2 & Hefs)".
+    iApply (step_fupdN_wand with "H"). iModIntro. iIntros "H".
+    iMod "H" as "(Hσ & He2 & Hefs)".
     iIntros "!>". rewrite Nat.add_comm app_length. iFrame.
   - iExists e, (t1' ++ e2' :: t2' ++ efs); iSplitR; first eauto.
-    iFrame "He". iDestruct "Ht" as "(Ht1 & He1 & Ht2)".
+    iDestruct "Ht" as "(Ht1 & He1 & Ht2)".
     iModIntro. iMod (wpc_step with "Hσ He1") as "H"; first done.
-    iIntros "!> !>". iMod "H" as "(Hσ & He2 & Hefs)". iIntros "!>".
-    rewrite !app_length /= !app_length.
+    iApply (step_fupdN_wand with "H"). iModIntro. iIntros "H".
+    iMod "H" as "(Hσ & He2 & Hefs)". iIntros "!>".
+    iFrame "He". rewrite !app_length /= !app_length.
     replace (length t1' + S (length t2' + length efs))
       with (length efs + (length t1' + S (length t2'))) by omega. iFrame.
 Qed.
 
-Lemma wptp_steps s n e1 t1 κs κs' t2 σ1 σ2 Φ Φc :
+Lemma wptp_steps s k n e1 t1 κs κs' t2 σ1 σ2 Φ Φc :
   nsteps n (e1 :: t1, σ1) κs (t2, σ2) →
-  state_interp σ1 (κs ++ κs') (length t1) -∗ WPC e1 @ s; ⊤; ∅ {{ Φ }} {{ Φc }} -∗ wptp s t1
-  ={⊤,∅}▷=∗^n ∃ e2 t2',
+  state_interp σ1 (κs ++ κs') (length t1) -∗ WPC e1 @ s; k; ⊤; ∅ {{ Φ }} {{ Φc }} -∗ wptp s k t1 -∗
+  |={⊤,⊤}_(2 * (S (S k)))=>^n (∃ e2 t2',
     ⌜t2 = e2 :: t2'⌝ ∗
     state_interp σ2 κs' (pred (length t2)) ∗
-    WPC e2 @ s; ⊤; ∅ {{ Φ }} {{ Φc }} ∗ wptp s t2'.
+    WPC e2 @ s; k; ⊤; ∅ {{ Φ }} {{ Φc }} ∗ wptp s k t2').
 Proof.
   revert e1 t1 κs κs' t2 σ1 σ2; simpl.
   induction n as [|n IH]=> e1 t1 κs κs' t2 σ1 σ2 /=.
@@ -64,25 +74,33 @@ Proof.
   iIntros (Hsteps) "Hσ He Ht". inversion_clear Hsteps as [|?? [t1' σ1']].
   rewrite -(assoc_L (++)).
   iMod (wptp_step with "Hσ He Ht") as (e1' t1'' ?) ">H"; first eauto; simplify_eq.
-  iIntros "!> !>". iMod "H" as "(Hσ & He & Ht)". iModIntro.
+  iApply (step_fupdN_wand with "H"). iModIntro. iIntros "H".
+  iMod "H" as "(Hσ & He & Ht)". iIntros "!>".
   by iApply (IH with "Hσ He Ht").
 Qed.
 
-Lemma wpc_safe κs m e σ Φ Φc :
+Lemma wpc_safe k κs m e σ Φ Φc :
   state_interp σ κs m -∗
-  WPC e {{ Φ }} {{ Φc }} ={⊤}=∗ ⌜is_Some (to_val e) ∨ reducible e σ⌝.
+  WPC e @ k {{ Φ }} {{ Φc }} ={⊤}=∗ ▷^(S (S k))
+  ⌜is_Some (to_val e) ∨ reducible e σ⌝.
 Proof.
   rewrite wpc_unfold /wpc_pre. iIntros "Hσ (H&_)".
   destruct (to_val e) as [v|] eqn:?; first by eauto.
-  iSpecialize ("H" $! σ [] κs with "Hσ"). rewrite sep_elim_l.
-  iMod (fupd_plain_mask with "H") as %?; eauto.
+  iSpecialize ("H" $! σ [] κs with "Hσ").
+  iMod (step_fupdN_inner_plain with "[H]") as "H".
+  2: { iMod "H". iApply (step_fupdN_wand with "H").
+       iModIntro. iIntros "(H&_)". iMod "H" as "(H&_)".
+       iApply "H". }
+  { apply _. }
+  iModIntro; eauto.
+  repeat iNext; iDestruct "H" as %?; eauto.
 Qed.
 
-Lemma wptp_strong_adequacy Φ Φc κs' s n e1 t1 κs t2 σ1 σ2 :
+Lemma wptp_strong_adequacy Φ Φc k κs' s n e1 t1 κs t2 σ1 σ2 :
   nsteps n (e1 :: t1, σ1) κs (t2, σ2) →
   state_interp σ1 (κs ++ κs') (length t1) -∗
-  WPC e1 @ s; ⊤; ∅ {{ Φ }} {{ Φc }} -∗
-  wptp s t1 ={⊤,∅}▷=∗^(S n) (∃ e2 t2',
+  WPC e1 @ s; k; ⊤; ∅ {{ Φ }} {{ Φc }} -∗
+  wptp s k t1 -∗ |={⊤,⊤}_(2 * (S (S k)))=>^(S n) (∃ e2 t2',
     ⌜ t2 = e2 :: t2' ⌝ ∗
     ⌜ ∀ e2, s = NotStuck → e2 ∈ t2 → (is_Some (to_val e2) ∨ reducible e2 σ2) ⌝ ∗
     state_interp σ2 κs' (length t2') ∗
@@ -91,17 +109,22 @@ Lemma wptp_strong_adequacy Φ Φc κs' s n e1 t1 κs t2 σ1 σ2 :
 Proof.
   iIntros (Hstep) "Hσ He Ht". rewrite Nat_iter_S_r.
   iDestruct (wptp_steps with "Hσ He Ht") as "Hwp"; first done.
-  iApply (step_fupdN_wand with "Hwp").
+  iApply (step_fupdN_innerN_wand with "Hwp"); auto.
   iDestruct 1 as (e2' t2' ?) "(Hσ & Hwp & Ht)"; simplify_eq/=.
   iMod (fupd_plain_keep_l ⊤
-    ⌜ ∀ e2, s = NotStuck → e2 ∈ (e2' :: t2') → (is_Some (to_val e2) ∨ reducible e2 σ2) ⌝%I
-    (state_interp σ2 κs' (length t2') ∗ WPC e2' @ s; ⊤; ∅ {{ v, Φ v }} {{ Φc }} ∗ wptp s t2')%I
+    (▷^(S (S k)) ⌜ ∀ e2, s = NotStuck → e2 ∈ (e2' :: t2') → (is_Some (to_val e2) ∨ reducible e2 σ2) ⌝)%I
+    (state_interp σ2 κs' (length t2') ∗ WPC e2' @ s; k; ⊤; ∅ {{ v, Φ v }} {{ Φc }} ∗ wptp s k t2')%I
     with "[$Hσ $Hwp $Ht]") as "(Hsafe&Hσ&Hwp&Hvs)".
   { iIntros "(Hσ & Hwp & Ht)" (e' -> He').
     apply elem_of_cons in He' as [<-|(t1''&t2''&->)%elem_of_list_split].
     - iMod (wpc_safe with "Hσ Hwp") as "$"; auto.
     - iDestruct "Ht" as "(_ & He' & _)". by iMod (wpc_safe with "Hσ He'"). }
-  iApply step_fupd_fupd. iApply step_fupd_intro; first done. iNext.
+  iApply step_fupd_fupd. iApply step_fupd_intro; first done.
+  iMod (fupd_intro_mask' _ ∅) as "Hclo". auto.
+  do 5 (iModIntro). iMod "Hclo".
+  iApply step_fupdN_inner_fupd.
+  iApply (step_fupdN_inner_later); auto.
+  iNext.
   iExists _, _. iSplitL ""; first done. iFrame "Hsafe Hσ".
   iSplitL "Hwp".
   - destruct (to_val e2') as [v2|] eqn:He2'; last done.
@@ -109,36 +132,39 @@ Proof.
   - clear Hstep. iInduction t2' as [|e t2'] "IH"; csimpl; first by iFrame.
     iDestruct "Hvs" as "[Hv Hvs]". destruct (to_val e) as [v|] eqn:He.
     + apply of_to_val in He as <-. iMod (wpc_value_inv' with "Hv") as "$".
-      by iApply "IH".
-    + by iApply "IH".
+      by iApply ("IH" with "[$]").
+    + by iApply ("IH" with "[$]").
 Qed.
 
-Lemma wptp_strong_crash_adequacy Φ Φc κs' s n e1 t1 κs t2 σ1 σ2 :
+Lemma wptp_strong_crash_adequacy Φ Φc κs' s k n e1 t1 κs t2 σ1 σ2 :
   nsteps n (e1 :: t1, σ1) κs (t2, σ2) →
   state_interp σ1 (κs ++ κs') (length t1) -∗
-  WPC e1 @ s; ⊤; ∅ {{ Φ }} {{ Φc }} -∗
-  wptp s t1 ={⊤,∅}▷=∗^(S n) |={⊤, ∅}=> (∃ e2 t2',
+  WPC e1 @ s; k; ⊤; ∅ {{ Φ }} {{ Φc }} -∗
+  wptp s k t1 -∗ |={⊤,⊤}_(2 * S (S k))=>^(S n) |={⊤, ∅}_(S k)=> (∃ e2 t2',
     ⌜ t2 = e2 :: t2' ⌝ ∗
     Φc ∗ state_interp σ2 κs' (length t2')).
 Proof.
   iIntros (Hstep) "Hσ He Ht". rewrite Nat_iter_S_r.
   iDestruct (wptp_steps with "Hσ He Ht") as "Hwp"; first done.
-  iApply (step_fupdN_wand with "Hwp").
+  iApply (step_fupdN_innerN_wand with "Hwp"); auto.
   iDestruct 1 as (e2' t2' ?) "(Hσ & Hwp & Ht)"; simplify_eq/=.
   iMod (fupd_plain_keep_l ⊤
-    ⌜ ∀ e2, s = NotStuck → e2 ∈ (e2' :: t2') → (is_Some (to_val e2) ∨ reducible e2 σ2) ⌝%I
-    (state_interp σ2 κs' (length t2') ∗ WPC e2' @ s; ⊤; ∅ {{ v, Φ v }} {{ Φc }} ∗ wptp s t2')%I
+    (▷^(S (S k)) ⌜ ∀ e2, s = NotStuck → e2 ∈ (e2' :: t2') → (is_Some (to_val e2) ∨ reducible e2 σ2) ⌝)%I
+    (state_interp σ2 κs' (length t2') ∗ WPC e2' @ s; k; ⊤; ∅ {{ v, Φ v }} {{ Φc }} ∗ wptp s k t2')%I
     with "[$Hσ $Hwp $Ht]") as "(Hsafe&Hσ&Hwp&Hvs)".
   { iIntros "(Hσ & Hwp & Ht)" (e' -> He').
     apply elem_of_cons in He' as [<-|(t1''&t2''&->)%elem_of_list_split].
     - iMod (wpc_safe with "Hσ Hwp") as "$"; auto.
     - iDestruct "Ht" as "(_ & He' & _)". by iMod (wpc_safe with "Hσ He'"). }
-  iApply step_fupd_fupd. iApply step_fupd_intro; first done. iNext.
-  iModIntro. iExists _, _.
-  rewrite {1}wpc_unfold /wpc_pre.
-  iDestruct "Hwp" as "(_&Hwp)".
-  iMod ("Hwp" with "[$]") as "($&$)".
-  iModIntro; eauto.
+  iApply step_fupd_fupd. iApply step_fupd_intro; first done.
+  iMod (fupd_intro_mask' _ ∅) as "Hclo". auto.
+  do 5 (iModIntro). iMod "Hclo".
+  iApply step_fupdN_inner_fupd.
+  iApply (step_fupdN_inner_later); auto.
+  iNext. iModIntro.
+  iMod (wpc_crash with "Hwp") as "H".
+  iApply (step_fupdN_inner_wand _ _ (S k) with "H [-]"); eauto.
+  iIntros "($&?)". iExists _, _; eauto.
 Qed.
 End crash_adequacy.
 
@@ -153,24 +179,25 @@ Class perennialG (Λ : language) (CS: crash_semantics Λ) (T: ofeT) (Σ : gFunct
   perennial_invG: ∀ H t, @iris_invG _ _ (perennial_irisG H t) = H
 }.
 
-Definition wpr_pre `{perennialG Λ CS T Σ} (s : stuckness)
+Definition wpr_pre `{perennialG Λ CS T Σ} (s : stuckness) (k: nat)
     (wpr : invG Σ -d> pbundleG T Σ -d> coPset -d> expr Λ -d> expr Λ -d> (val Λ -d> iPropO Σ) -d>
                      (invG Σ -d> pbundleG T Σ -d> val Λ -d> iPropO Σ) -d> iPropO Σ) :
   invG Σ -d> pbundleG T Σ -d> coPset -d> expr Λ -d> expr Λ -d> (val Λ -d> iPropO Σ) -d> (invG Σ -d> pbundleG T Σ -d> val Λ -d> iPropO Σ) -d> iPropO Σ :=
   λ H t E e rec Φ Φr,
-  (WPC e @ s ; E ; ∅
+  (WPC e @ s ; k; E ; ∅
      {{ Φ }}
      {{ ∀ σ σ' (HC: crash_prim_step CS σ σ') κs n,
         state_interp σ κs n ={∅}=∗  ▷ ∀ H, ∃ t, state_interp σ' κs 0 ∗ wpr H t E rec rec (λ v, Φr H t v) Φr}})%I.
 
-Local Instance wpr_pre_contractive `{!perennialG Λ CS T Σ} s : Contractive (wpr_pre s).
+Local Instance wpr_pre_contractive `{!perennialG Λ CS T Σ} s k: Contractive (wpr_pre s k).
 Proof.
   rewrite /wpr_pre=> n wp wp' Hwp ? t E1 e1 rec Φ Φc.
-  repeat (f_contractive || f_equiv); apply Hwp.
+  apply wpc_ne; eauto;
+  repeat (f_contractive || f_equiv). apply Hwp.
 Qed.
 
-Definition wpr_def `{!perennialG Λ CS T Σ} (s : stuckness) :
-  invG Σ → pbundleG T Σ → coPset → expr Λ → expr Λ → (val Λ → iProp Σ) → (invG Σ → pbundleG T Σ → val Λ → iProp Σ) → iProp Σ := fixpoint (wpr_pre s).
+Definition wpr_def `{!perennialG Λ CS T Σ} (s : stuckness) k :
+  invG Σ → pbundleG T Σ → coPset → expr Λ → expr Λ → (val Λ → iProp Σ) → (invG Σ → pbundleG T Σ → val Λ → iProp Σ) → iProp Σ := fixpoint (wpr_pre s k).
 Definition wpr_aux `{!perennialG Λ CS T Σ} : seal (@wpr_def Λ CS T Σ _). by eexists. Qed.
 Definition wpr `{!perennialG Λ CS T Σ} := wpr_aux.(unseal).
 Definition wpr_eq `{!perennialG Λ CS T Σ} : wpr = @wpr_def Λ CS T Σ _ := wpr_aux.(seal_eq).
@@ -178,21 +205,22 @@ Definition wpr_eq `{!perennialG Λ CS T Σ} : wpr = @wpr_def Λ CS T Σ _ := wpr
 Section wpr.
 Context `{!perennialG Λ CS T Σ}.
 Implicit Types s : stuckness.
+Implicit Types k : nat.
 Implicit Types P : iProp Σ.
 Implicit Types Φ : val Λ → iProp Σ.
 Implicit Types Φc : invG Σ → pbundleG T Σ → val Λ → iProp Σ.
 Implicit Types v : val Λ.
 Implicit Types e : expr Λ.
 
-Lemma wpr_unfold s Hi t E e rec Φ Φc :
-  wpr s Hi t E e rec Φ Φc ⊣⊢ wpr_pre s (wpr s) Hi t E e rec Φ Φc.
-Proof. rewrite wpr_eq. apply (fixpoint_unfold (wpr_pre s)). Qed.
+Lemma wpr_unfold s k Hi t E e rec Φ Φc :
+  wpr s k Hi t E e rec Φ Φc ⊣⊢ wpr_pre s k (wpr s k) Hi t E e rec Φ Φc.
+Proof. rewrite wpr_eq. apply (fixpoint_unfold (wpr_pre s k)). Qed.
 
 (* There's a stronger version of this *)
-Lemma wpr_strong_mono s Hi t E e rec Φ Ψ Φr Ψr :
-  wpr s Hi t E e rec Φ Φr -∗
+Lemma wpr_strong_mono s k Hi t E e rec Φ Ψ Φr Ψr :
+  wpr s k Hi t E e rec Φ Φr -∗
   (∀ v, Φ v ==∗ Ψ v) ∧ (∀ Hi t v, Φr Hi t v ==∗ Ψr Hi t v) -∗
-  wpr s Hi t E e rec Ψ Ψr.
+  wpr s k Hi t E e rec Ψ Ψr.
 Proof.
   iIntros "H HΦ". iLöb as "IH" forall (e t Hi E Φ Ψ Φr Ψr).
   rewrite ?wpr_unfold /wpr_pre.
@@ -208,17 +236,17 @@ Qed.
 
 (* To prove a recovery wp for e with rec, it suffices to prove a crash wp for e,
    where the crash condition implies the precondition for a crash wp for rec *)
-Lemma idempotence_wpr s E e rec Φx Φrx Φcx Hi t:
-  ((WPC e @ s ; E ; ∅ {{ Φx t }} {{ Φcx t }}) -∗
+Lemma idempotence_wpr s k E e rec Φx Φrx Φcx Hi t:
+  ((WPC e @ s ; k ; E ; ∅ {{ Φx t }} {{ Φcx t }}) -∗
    (□ ∀ (H: invG Σ) (t: pbundleG T Σ) σ σ' (HC: crash_prim_step CS σ σ') κs n,
         Φcx t -∗ state_interp σ κs n ={∅}=∗
-        ▷ ∀ H', ∃ t', state_interp σ' κs 0 ∗ WPC rec @ s ; E ; ∅ {{ Φrx H' t' }} {{ Φcx t' }}) -∗
-    wpr s Hi t E e rec (Φx t) Φrx)%I.
+        ▷ ∀ H', ∃ t', state_interp σ' κs 0 ∗ WPC rec @ s ; k; E ; ∅ {{ Φrx H' t' }} {{ Φcx t' }}) -∗
+    wpr s k Hi t E e rec (Φx t) Φrx)%I.
 Proof.
   iLöb as "IH" forall (E e Hi t Φx).
   iIntros "He #Hidemp".
   rewrite wpr_unfold. rewrite /wpr_pre.
-  iApply (wpc_strong_mono with "He"); [ auto | auto | auto | ].
+  iApply (wpc_strong_mono with "He"); [ auto | auto | auto | auto | ].
   iSplit; first auto. iIntros "Hcx". iModIntro.
   iIntros. iMod ("Hidemp" with "[ ] [$] [$]") as "H".
   { eauto. }
@@ -234,48 +262,63 @@ End wpr.
 Section recovery_adequacy.
 Context `{!perennialG Λ CS T Σ}.
 Implicit Types s : stuckness.
+Implicit Types k : nat.
 Implicit Types P : iProp Σ.
 Implicit Types Φ : val Λ → iProp Σ.
 Implicit Types Φc : invG Σ → pbundleG T Σ → val Λ → iProp Σ.
 Implicit Types v : val Λ.
 Implicit Types e : expr Λ.
 
-Notation wptp s t := ([∗ list] ef ∈ t, WPC ef @ s; ⊤; ∅ {{ fork_post }} {{ True }})%I.
+Notation wptp s k t := ([∗ list] ef ∈ t, WPC ef @ s; k; ⊤; ∅ {{ fork_post }} {{ True }})%I.
 
-Fixpoint step_fupdN_fresh (ns: list nat) Hi0 t0 (P: invG Σ → pbundleG T Σ → iProp Σ) :=
+Fixpoint step_fupdN_fresh k (ns: list nat) Hi0 t0 (P: invG Σ → pbundleG T Σ → iProp Σ) :=
   match ns with
   | [] => P Hi0 t0
   | (n :: ns) =>
-    (|={⊤, ∅}▷=>^(S n) |={⊤, ∅}=> ▷
-     ∀ Hi', (∃ t' : pbundleG T Σ, step_fupdN_fresh ns Hi' t' P))%I
+    (|={⊤, ⊤}_k=>^(S n) |={⊤, ∅}_k=> ▷
+     ∀ Hi', (∃ t' : pbundleG T Σ, step_fupdN_fresh k ns Hi' t' P))%I
   end.
 
-Lemma step_fupdN_fresh_snoc (ns: list nat) n Hi0 t0 Q:
-  step_fupdN_fresh (ns ++ [n]) Hi0 t0 Q ≡
-  step_fupdN_fresh (ns) Hi0 t0
-    (λ Hi _, |={⊤, ∅}▷=>^(S n) |={⊤, ∅}=> ▷ ∀ Hi', ∃ t', Q Hi' t')%I.
+Lemma step_fupdN_fresh_snoc k (ns: list nat) n Hi0 t0 Q:
+  step_fupdN_fresh k (ns ++ [n]) Hi0 t0 Q ≡
+  step_fupdN_fresh k (ns) Hi0 t0
+    (λ Hi _, |={⊤, ⊤}_k=>^(S n) |={⊤, ∅}_k=> ▷ ∀ Hi', ∃ t', Q Hi' t')%I.
 Proof.
   apply (anti_symm (⊢)%I).
   - revert Hi0 t0 Q.
-    induction ns => ??? //=. do 3 f_equiv.
-    apply step_fupdN_mono.
-    do 2 f_equiv. do 2 (f_equiv => ?).
-    rewrite IHns. eauto.
+    induction ns => ??? //=. do 1 f_equiv.
+    apply step_fupdN_mono. apply fupd_mono.
+    iIntros "H".
+    iApply (step_fupdN_innerN_wand with "H"); auto.
+    iIntros "H".
+    iApply (step_fupdN_inner_wand' with "H"); auto.
+    iIntros "H". iNext. iIntros.
+    iDestruct ("H" $! _) as (?) "H".
+    iExists _. by iApply IHns.
   - revert Hi0 t0 Q.
-    induction ns => ??? //=. do 3 f_equiv.
-    apply step_fupdN_mono.
-    do 2 f_equiv. do 2 (f_equiv => ?).
-    rewrite IHns. eauto.
+    induction ns => ??? //=. do 1 f_equiv.
+    apply step_fupdN_mono. apply fupd_mono.
+    iIntros "H".
+    iApply (step_fupdN_innerN_wand with "H"); auto.
+    iIntros "H".
+    iApply (step_fupdN_inner_wand' with "H"); auto.
+    iIntros "H". iNext. iIntros.
+    iDestruct ("H" $! _) as (?) "H".
+    iExists _. by iApply IHns.
 Qed.
 
-Lemma step_fupdN_fresh_pattern_wand {H: invG Σ} n (Q Q': iProp Σ):
-  (|={⊤, ∅}▷=>^(S n) |={⊤, ∅}=> ▷ Q) -∗ (Q -∗ Q') -∗
-  (|={⊤, ∅}▷=>^(S n) |={⊤, ∅}=> ▷ Q').
+Lemma step_fupdN_fresh_pattern_wand {H: invG Σ} k n (Q Q': iProp Σ):
+  (|={⊤, ⊤}_k=>^(S n) |={⊤, ∅}_k=> ▷ Q) -∗ (Q -∗ Q') -∗
+  (|={⊤, ⊤}_k=>^(S n) |={⊤, ∅}_k=> ▷ Q').
 Proof.
   iIntros "H Hwand". simpl.
   iApply (step_fupdN_wand with "H").
-  iNext. iIntros "H".
-  iMod "H". iModIntro. iNext.
+  iIntros "H". iMod "H". iModIntro.
+  iApply (step_fupdN_innerN_wand with "H"); auto.
+  iIntros "H".
+  iApply (step_fupdN_inner_wand' with "H"); auto.
+  iIntros "H".
+  iNext.
   by iApply "Hwand".
 Qed.
 
@@ -291,9 +334,24 @@ Proof.
   iMod "H". iModIntro. iNext. rewrite -later_laterN laterN_later. iNext. by iMod "H".
 Qed.
 
-Lemma step_fupdN_fresh_wand (ns: list nat) Hi0 t0 Q Q':
-  step_fupdN_fresh (ns) Hi0 t0 Q -∗ (∀ Hinv t, Q Hinv t -∗ Q' Hinv t)
-  -∗ step_fupdN_fresh ns Hi0 t0 Q'.
+Lemma step_fupdN_fresh_pattern_plain' {H: invG Σ} k n (Q: iProp Σ) `{!Plain Q}:
+  (|={⊤, ⊤}_k=>^(S n) |={⊤, ∅}_k=> ▷ Q) -∗
+  (|={⊤}=> ▷^(S (S n) * (S (S k))) Q).
+Proof.
+  iIntros "H".
+  iDestruct (step_fupdN_innerN_wand with "H []") as "H"; auto.
+  { iApply step_fupdN_inner_plain. }
+  rewrite step_fupdN_innerN_S_fupd.
+  iMod (step_fupdN_innerN_plain with "H") as "H".
+  iModIntro.
+  replace (S (S n) * (S (S k))) with (S n * (S (S k)) + S (S k)) by lia.
+  rewrite laterN_plus. iApply (laterN_le (S n * S k)); first by lia.
+  iNext. rewrite -laterN_later => //=.
+Qed.
+
+Lemma step_fupdN_fresh_wand k (ns: list nat) Hi0 t0 Q Q':
+  step_fupdN_fresh k (ns) Hi0 t0 Q -∗ (∀ Hinv t, Q Hinv t -∗ Q' Hinv t)
+  -∗ step_fupdN_fresh k ns Hi0 t0 Q'.
 Proof.
   revert Hi0 t0.
   induction ns => ??.
@@ -305,55 +363,55 @@ Proof.
     iExists _. iApply (IHns with "H"). eauto.
 Qed.
 
-Fixpoint fresh_later_count (ns: list nat) :=
+Fixpoint fresh_later_count k (ns: list nat) :=
   match ns with
-  | [] => 2
-  | n :: ns' => (S (S n)) + fresh_later_count ns'
+  | [] => (S (S k))
+  | n :: ns' => (S (S n) * (S (S k))) + fresh_later_count k ns'
   end.
 
-Lemma step_fupdN_fresh_plain `{!invPreG Σ} P `{!Plain P} ns n:
-  (∀ Hinv', |={⊤}=> ∃ t, step_fupdN_fresh ns Hinv' t
-                  (λ _ _, |={⊤, ∅}▷=>^(S n) |={⊤, ∅}=> P)) -∗
-  ▷^(fresh_later_count ns + n) P.
+Lemma step_fupdN_fresh_plain `{!invPreG Σ} P `{!Plain P} k ns n:
+  (∀ Hinv', |={⊤}=> ∃ t, step_fupdN_fresh k ns Hinv' t
+                  (λ _ _, |={⊤, ⊤}_k=>^(S n) |={⊤, ∅}=> P)) -∗
+  ▷^(fresh_later_count k ns + S (S k + n * (S (S k)))) P.
 Proof.
   iIntros "H".
   iInduction ns as [| n' ns] "IH".
   - rewrite /step_fupdN_fresh.
-    iApply (bupd_plain (▷^((S (S n))) P)%I); try (iPureIntro; apply _).
+    iApply (bupd_plain (▷^(_) P)%I); try (iPureIntro; apply _).
     iMod wsat_alloc as (Hinv) "(Hw&HE)".
     iSpecialize ("H" $! Hinv).
     rewrite {1}uPred_fupd_eq {1}/uPred_fupd_def.
     iMod ("H" with "[$]") as "[>Hw [>HE >H]]".
     iDestruct ("H") as (_) "H".
-    iDestruct (step_fupdN_fresh_pattern_plain _ (P)%I with "[H]") as "H".
-    iApply (step_fupdN_wand with "H").
-    { iIntros "H". iMod "H". iModIntro. by iNext. }
+    iDestruct (step_fupdN_fresh_pattern_plain' _ _ (P)%I with "[H]") as "H".
+    iApply (step_fupdN_innerN_wand with "H"); try reflexivity.
+    { iIntros "H". iMod "H". iApply step_fupdN_inner_later; auto. }
     rewrite {1}uPred_fupd_eq {1}/uPred_fupd_def.
-    by iMod ("H" with "[$]") as "[Hw [HE >$]]".
+    iMod ("H" with "[$]") as "[Hw [HE >$]]"; eauto.
   - iMod wsat_alloc as (Hinv) "(Hw&HE)".
     iSpecialize ("H" $! Hinv).
     rewrite {1}uPred_fupd_eq {1}/uPred_fupd_def.
     iMod ("H" with "[$]") as "[>Hw [>HE >H]]".
     iDestruct "H" as (t) "H".
     rewrite /step_fupdN_fresh -/step_fupdN_fresh.
-    iDestruct (step_fupdN_fresh_pattern_wand  _ _
-                 (▷^(fresh_later_count ns + n) P)
+    iDestruct (step_fupdN_fresh_pattern_wand  _ _ _
+                  (▷^(fresh_later_count k ns + _) P)
                  with "H [IH]") as "H".
     { iIntros "H". iApply "IH". iIntros. iModIntro. iApply "H". }
-    iDestruct (step_fupdN_fresh_pattern_plain with "H") as "H".
+    iDestruct (step_fupdN_fresh_pattern_plain' with "H") as "H".
     rewrite {1}uPred_fupd_eq {1}/uPred_fupd_def.
     iMod ("H" with "[$]") as "[Hw [HE >H]]".
-    simpl.
-    by rewrite ?laterN_plus.
+    simpl. rewrite ?laterN_plus. iApply "H".
 Qed.
 
-Lemma step_fupdN_fresh_soundness `{!invPreG Σ} (φ : Prop) ns n:
-  (∀ Hinv : invG Σ, (|={⊤}=> (∃ t0, step_fupdN_fresh ns Hinv t0
-                             (λ _ _, |={⊤, ∅}▷=>^(S n) |={⊤, ∅}=> ▷ ⌜φ⌝)))%I) →
+(* XXX this probably needs to be tweaked. *)
+Lemma step_fupdN_fresh_soundness `{!invPreG Σ} (φ : Prop) k ns n:
+  (∀ Hinv : invG Σ, (|={⊤}=> (∃ t0, step_fupdN_fresh k ns Hinv t0
+                             (λ _ _, |={⊤, ⊤}_k=>^(S n) |={⊤, ∅}=> ▷ ⌜φ⌝)))%I) →
   φ.
 Proof.
   intros Hiter.
-  apply (soundness (M:=iResUR Σ) _  (fresh_later_count ns + n + 1)); simpl.
+  eapply (soundness (M:=iResUR Σ) _  (fresh_later_count k ns + _ + 1)); simpl.
   rewrite laterN_plus.
   iApply step_fupdN_fresh_plain. iIntros (Hinv). iApply Hiter.
 Qed.
@@ -365,13 +423,13 @@ Notation "P ={ E }=∗_ t Q" := (P -∗ |={E}=>_(t) Q)%I
  (at level 99) : bi_scope.
 *)
 
-Lemma wptp_recv_strong_normal_adequacy Φ Φr κs' s Hi t n ns r1 e1 t1 κs t2 σ1 σ2 :
+Lemma wptp_recv_strong_normal_adequacy Φ Φr κs' s k Hi t n ns r1 e1 t1 κs t2 σ1 σ2 :
   nrsteps (CS := CS) r1 (ns ++ [n]) (e1 :: t1, σ1) κs (t2, σ2) Normal →
   state_interp σ1 (κs ++ κs') (length t1) -∗
-  wpr s Hi t ⊤ e1 r1 Φ Φr -∗
-  wptp s t1 -∗ step_fupdN_fresh ns Hi t (λ Hi' t',
+  wpr s k Hi t ⊤ e1 r1 Φ Φr -∗
+  wptp s k t1 -∗ step_fupdN_fresh (2 * (S (S k))) ns Hi t (λ Hi' t',
     ⌜ Hi' = Hi ∧ t' = t ⌝ ∗
-    (|={⊤, ∅}▷=>^(S n) |={⊤, ∅}=> ▷ ∃ e2 t2',
+    (|={⊤, ⊤}_(2 * (S (S k)))=>^(S n) |={⊤, ∅}=> ▷ ∃ e2 t2',
     ⌜ t2 = e2 :: t2' ⌝ ∗
     ⌜ ∀ e2, s = NotStuck → e2 ∈ t2 → (is_Some (to_val e2) ∨ reducible e2 σ2) ⌝ ∗
     state_interp σ2 κs' (length t2') ∗
@@ -389,17 +447,17 @@ Proof.
   rewrite /step_fupdN_fresh.
   rewrite perennial_invG.
   iSplitL ""; first by eauto.
-  iApply (step_fupdN_wand with "H").
+  iApply (step_fupdN_innerN_wand with "H"); auto.
   iIntros. iApply fupd_mask_weaken; first by set_solver+.
   iNext. eauto.
 Qed.
 
-Lemma wptp_recv_strong_crash_adequacy Φ Φr κs' s Hi t ns n r1 e1 t1 κs t2 σ1 σ2 :
+Lemma wptp_recv_strong_crash_adequacy Φ Φr κs' s k Hi t ns n r1 e1 t1 κs t2 σ1 σ2 :
   nrsteps (CS := CS) r1 (ns ++ [n]) (e1 :: t1, σ1) κs (t2, σ2) Crashed →
   state_interp σ1 (κs ++ κs') (length t1) -∗
-  wpr s Hi t ⊤ e1 r1 Φ Φr -∗
-  wptp s t1 -∗ step_fupdN_fresh ns Hi t (λ Hi' t',
-    (|={⊤, ∅}▷=>^(S n) |={⊤, ∅}=> ▷ ∃ e2 t2',
+  wpr s k Hi t ⊤ e1 r1 Φ Φr -∗
+  wptp s k t1 -∗ step_fupdN_fresh (2 * (S (S k))) ns Hi t (λ Hi' t',
+    (|={⊤, ⊤}_(2 * (S (S k)))=>^(S n) |={⊤, ∅}=> ▷ ∃ e2 t2',
     ⌜ t2 = e2 :: t2' ⌝ ∗
     ⌜ ∀ e2, s = NotStuck → e2 ∈ t2 → (is_Some (to_val e2) ∨ reducible e2 σ2) ⌝ ∗
     state_interp σ2 κs' (length t2') ∗
@@ -418,12 +476,19 @@ Proof.
   inversion_clear Hsteps as [|?? [t1' σ1'] ????? s0].
   rewrite {1}/step_fupdN_fresh -/step_fupdN_fresh.
   destruct ρ2 as (?&σ2_pre_crash).
-  iApply (step_fupdN_wand with "[-]").
+  iApply (step_fupdN_innerN_wand with "[-]"); try reflexivity.
   { rewrite -assoc wpr_unfold /wpr_pre.
     iPoseProof (@wptp_strong_crash_adequacy with "[$] [$]") as "H"; eauto.
     rewrite perennial_invG. by iApply "H".
   }
-  iIntros "H". iMod "H" as (e2 t2' ?) "(H&Hσ)".
+  iIntros "H".
+  rewrite -step_fupdN_inner_fupd.
+  iApply (step_fupdN_inner_wand' with "H").
+  { reflexivity. }
+  { reflexivity. }
+  { lia. }
+  iIntros "H".
+  iDestruct "H" as (e2 t2' ?) "(H&Hσ)".
   iMod ("H" with "[//] Hσ") as "H". iModIntro. iNext.
   destruct s0.
   - iIntros (Hi'). iSpecialize ("H" $! Hi').
@@ -439,12 +504,12 @@ Proof.
     iApply "H".
 Qed.
 
-Lemma wptp_recv_strong_adequacy Φ Φr κs' s Hi t ns n r1 e1 t1 κs t2 σ1 σ2 stat :
+Lemma wptp_recv_strong_adequacy Φ Φr κs' s k Hi t ns n r1 e1 t1 κs t2 σ1 σ2 stat :
   nrsteps (CS := CS) r1 (ns ++ [n]) (e1 :: t1, σ1) κs (t2, σ2) stat →
   state_interp σ1 (κs ++ κs') (length t1) -∗
-  wpr s Hi t ⊤ e1 r1 Φ Φr -∗
-  wptp s t1 -∗ step_fupdN_fresh ns Hi t (λ Hi' t',
-    (|={⊤, ∅}▷=>^(S n) |={⊤, ∅}=> ▷ ∃ e2 t2',
+  wpr s k Hi t ⊤ e1 r1 Φ Φr -∗
+  wptp s k t1 -∗ step_fupdN_fresh (2 * (S (S k))) ns Hi t (λ Hi' t',
+    (|={⊤, ⊤}_(2 * (S (S k)))=>^(S n) |={⊤, ∅}=> ▷ ∃ e2 t2',
     ⌜ t2 = e2 :: t2' ⌝ ∗
     ⌜ ∀ e2, s = NotStuck → e2 ∈ t2 → (is_Some (to_val e2) ∨ reducible e2 σ2) ⌝ ∗
     state_interp σ2 κs' (length t2') ∗
@@ -460,7 +525,7 @@ Proof.
     iApply (step_fupdN_fresh_wand with "H").
     iIntros (??) "H".
     iDestruct "H" as ((?&?)) "H". subst.
-    iApply (step_fupdN_wand with "H").
+    iApply (step_fupdN_innerN_wand with "H"); auto.
     iIntros ">H !> !> ".
     iDestruct "H" as (????) "(H&?&?)". iExists _, _.
     repeat (iSplitL ""; try iFrame; eauto).
@@ -497,7 +562,7 @@ Proof.
   - constructor; naive_solver.
 Qed.
 
-Corollary wp_recv_adequacy Σ Λ CS (T: ofeT) `{!invPreG Σ} s e r σ φ φr :
+Corollary wp_recv_adequacy Σ Λ CS (T: ofeT) `{!invPreG Σ} s k e r σ φ φr :
   (∀ `{Hinv : !invG Σ} κs,
      (|={⊤}=> ∃ (t: pbundleG T Σ)
          (stateI : pbundleG T Σ→ state Λ → list (observation Λ) → iProp Σ)
@@ -508,14 +573,14 @@ Corollary wp_recv_adequacy Σ Λ CS (T: ofeT) `{!invPreG Σ} s e r σ φ φr :
                IrisG Λ Σ Hi (λ σ κs _, stateI t σ κs)
                     (fork_post t)) Hpf
                in
-       stateI t σ κs ∗ wpr s Hinv t ⊤ e r (λ v, ⌜φ v⌝) (λ _ _ v, ⌜φr v⌝))%I) →
+       stateI t σ κs ∗ wpr s k Hinv t ⊤ e r (λ v, ⌜φ v⌝) (λ _ _ v, ⌜φr v⌝))%I) →
   recv_adequate (CS := CS) s e r σ (λ v _, φ v) (λ v _, φr v) .
 Proof.
   intros Hwp.
   apply recv_adequate_alt.
   intros t2 σ2 stat [n [κs H]]%erased_rsteps_nrsteps.
   destruct (nrsteps_snoc _ _ _ _ _ _ H) as (ns'&n'&->).
-  eapply (step_fupdN_fresh_soundness _ ns' n')=> Hinv.
+  eapply (step_fupdN_fresh_soundness _ (2 * (S (S k))) ns' n')=> Hinv.
   iMod (Hwp Hinv κs) as (t stateI Hfork_post Hpf) "(Hw&H)".
   iModIntro. iExists _.
   iDestruct (wptp_recv_strong_adequacy
@@ -527,7 +592,7 @@ Proof.
   { rewrite app_nil_r. eauto. }
   iApply (step_fupdN_fresh_wand with "H").
   iIntros (??) "H".
-  iApply (step_fupdN_mono with "H").
+  iApply (step_fupdN_innerN_wand with "H"); auto.
   iIntros ">H !> !> ".
   iDestruct "H" as (v2 ???) "(_&Hv&Hnstuck)".
   iSplitR ""; last done.
